\documentclass{article} 
\title{tasks 1}
\begin{document} 
\maketitle
\LARGE{\centerline{Exercise 1.}}
\Large{\leftline{A)}}
\Large{\leftline{$(1 + x^4)yy'$ - $x^3(y^2 + 1) = 0 $}}
\Large{\leftline{$ Y(1)=1 $}}
\Large{\leftline{$(1 + x^4)yy'$ - $x^3(y^2 + 1) = 0 =>$}
\leftline{$ => (1 + x^4)y\frac{dy}{dx}$ - $x^3(y^2 + 1) = 0 =>$}
\leftline{$ => (1 + x^4)y\frac{dy}{dx} = x^3y^2 + x^3 =>$}
\leftline{$ => (1 + x^4)\frac{dy}{dx} = x^3y + \frac{x^3}{y}  =>$}
\leftline{$ => (1 + x^4)\frac{dy}{dx} = x^3( y + \frac{1}{y})  =>$}
\leftline{$ => (1 + x^4)\frac{dy}{dx} = x^3\frac{y ^2 + 1}{y}  =>$}
\leftline{$ => \frac{y}{y ^2 + 1}by = \frac{x^3}{1 + x^4}dx  =>$}
\leftline{$ => \int \frac{y}{y ^2 + 1}by = \int \frac{x^3}{1 + x^4}dx +c =>$}
\leftline{$ => \frac{1}{2}\int \frac{2y}{y ^2 + 1}by = \frac{1}{4}\int \frac{4x^3}{1 + x^4}dx +c =>$}
\leftline{$ => \frac{1}{2}ln|y ^2 + 1| = \frac{1}{4}ln|1 + x^4| +c =>(1)$}
\centerline{$y ^2 + 1 > 0(2)$              $1 + x^4 > 0 (3) $}
\leftline{$(1)(2)(3)=>\frac{1}{2}ln(y ^2 + 1) = \frac{1}{4}ln(1 + x^4) +c =>$}
\leftline{$ => ln(y ^2 + 1) = \frac{1}{2}ln(1 + x^4) +2c =>$}
\leftline{$ => y ^2 + 1 = e^{\frac{1}{2}ln(1 + x^4)}e^{2c} =>$}
\leftline{$ => y ^2  = e^{ln(\sqrt{1 + x^4})}e^{2c} - 1 =>$}
\leftline{$ => y ^2  = \sqrt{1 + x^4}e^{2c} - 1 =^{(e^{2c}=K)}=> $}
\leftline{$ => y ^2  = \sqrt{1 + x^4}K - 1 => (4) $}
\leftline{$Y(1) = 1 =>1 = \sqrt{2}K -1 => 2 = \sqrt{2}K => \frac{2\sqrt{2}}{2} = K =>$}
\leftline{$=> K=\sqrt{2} => (5)$}
\leftline{$(5)(4)=>y ^2  = \sqrt{1 + x^4}\sqrt{2} - 1 => $}
\leftline{$y ^2  = \sqrt{2 + 2x^4} - 1 => $}
\leftline{$ =>y  =  \sqrt{\sqrt{2 + 2x^4} - 1} $}
}
\LARGE{\leftline{B)}}
\Large{\leftline{$y'=\frac{2xy - y^2}{3x^2 + 2xy}$}
\leftline{$y' = \frac{dy}{dx} = \frac{2\frac{y}{x} + (\frac{y}{x})^2}{3 + 2\frac{y}{x}} = $}
\leftline{$=^{(u=\frac{y}{x})}= \frac{2u + u^2}{3 + 2u} = (1) $}
\leftline{$y = xu => y' = u + xu' (2) $}
\leftline{$ (1)(2) =>u + xu' = \frac{2u + u^2}{3 + 2u} => $}
\leftline{$ => \frac{du}{dx} = \frac{2u + u^2}{3x + 2ux} $ - $\frac{u}{x}=> $}
\leftline{$ => \frac{du}{dx} = \frac{2u + u^2 - u(3 + 2u)}{x(3 + 2u)} =>$}
\leftline{$ => \frac{du}{dx} = \frac{-u - u^2}{x(3 + 2u)} =>$}
\leftline{$ => \frac{3 + 2u}{-u - u^2}du = \frac{1}{x}dx =>$}
\leftline{$ => -\int\frac{3 + 2u}{u + u^2}du = \int\frac{1}{x}dx +c=>$}
\leftline{$ => -\int\frac{3 + 2u}{u(1 + u)}du = \int\frac{1}{x}dx +c=>(3)$}
\leftline{$\frac{3 + 2u}{u(1 + u)} = \frac{A}{u} + \frac{B}{(1 + u)} =>$}
\leftline{$ =>3 + 2u = A(1 + u) + Bu => 3 + 2u = u(A + B) + A => $}
\centerline{$A = 3 (4) $}
\centerline{$A + B = 2 => B = -1 (5)$}
\leftline{$ (3)(4)(5)=> -\int\frac{3}{u} + \frac{-1}{(1 + u)}du = \int\frac{1}{x}dx +c => $}
\leftline{$ => -3ln|u| + ln|1 + u| = ln|x| +c => $}
\leftline{$ => |\frac{u + 1}{xu^3}| = e^c =^{(\pm e^c = K)}=> \frac{u + 1}{u^3} = Kx => $}
\leftline{$ => \frac{\frac{y + x}{x}}{(\frac{y}{x})^3} = Kx =>  $}
\leftline{$ => \frac{x(y + x)}{(y)^3} = K =>  \frac{(y + x)}{(y)^3} = \frac{K}{x}$}
}
\LARGE{\centerline{Exercise 2.}}
\LARGE{\leftline{A)}}
\Large{\leftline{$ (3xy + y^2) + (x^2 + yx)y'= 0 $}}
\Large{\leftline{$ x > 0 $}}
\Large{\leftline{$(3xy + y^2)dx + (x^2 + yx)dy = 0 =>(1)$}
\leftline{$M(x,y) = 3xy + y^2 $ and $ N(x,y) = x^2 + yx$} 
\leftline{$ \frac{\partial M(x,y)}{\partial y} = \frac{\partial}{\partial y}(3xy + y^2) = 3x + 2y $}
\leftline{$ \frac{\partial N(x,y)}{\partial x} = \frac{\partial}{\partial x}(x^2 + xy) = 2x + y $}
\leftline{$ 3x + 2y = 2x + y => x = -y $ the DE is not accurate }
\leftline{$ \frac{M_y - N_x}{N} = \frac{3x + 2y - 2x - y}{x^2 + xy} = \frac{x + y}{x(x + y)} = \frac{1}{x} $}
\leftline{$( r(u_1) = \frac{1}{x} )$        $ (u_1 = x)$}
\leftline{$ m(x) = e^{\int r(u_1) du} = e^{\int \frac{1}{x} du} = e^{ln|x|} = |x| =^{(x>0)}= x$}
\leftline{$(1) => (3xy + y^2)dx + (x^2 + yx)dy = 0 =>$}
\leftline{$ => (3x^2y + y^2x)dx + (x^3 + x^2y)dy = 0 $}
\leftline{$M(x,y) = 3x^2y + y^2x $ and $ N(x,y) = x^3 + x^2y$}
\leftline{$ M_y = 3x^2 + 2yx$ and $N_x = 3x^2 + 2xy$}
\leftline{$ M_y = N_x = 3x^2 + 2xy$ the DE is accurate}
\leftline{$ \frac{\partial u}{\partial x} = M(x,y) = 3x^2y + y^2x $}
\leftline{$ \frac{\partial u}{\partial x} = N(x,y) = x^3 + x^2y =>(3)$}
\leftline{$ u = \int \frac{\partial u}{\partial x} dx = \int  3x^2y + y^2x dx = x^3y + y^2x^2\frac{1}{2} + K(y) => (2)$}
\leftline{$ \frac{\partial u}{\partial x} =^{(2)}= \frac{\partial }{\partial x}(x^3y + y^2x^2\frac{1}{2} + K(y)) =^{(3)}=> $}
\leftline{$ =^{(3)}=>x^3 + x^2y = x^3 + x^2y + K'(y) => K'(y) = 0 => K(y) = c $}
\leftline{$ (2)=> u(x,y) = x^3y + y^2x^2\frac{1}{2} + c => (4)$}
\leftline{$ u(x,y) = sta = c_2 =>(5)$}
\leftline{$ (4)(5)=> c_2 = x^3y + y^2x^2\frac{1}{2} + c =^{(c_3 = c_2 - c)}=>$}
\leftline{$ => x^3y + y^2x^2\frac{1}{2} = c_3 =>$}
\leftline{$ => 2x^3y + y^2x^2 = 2c_3 =>$}
\leftline{$ => 2xy + y^2 = \frac{2c_3}{x^2} =>$}
\leftline{$ => x^2 + 2xy + y^2 = \frac{2c_3}{x^2} + x^2 =>$}
\leftline{$ =>  (y + x)^2 = \frac{2c_3}{x^2} + x^2 =>$}
\leftline{$ => y + x = \pm \sqrt{\frac{2c_3}{x^2} + x^2} =>$}
\leftline{$  y  = - x \pm \sqrt{\frac{2c_3}{x^2} + x^2} $}
\leftline{$c_3 \geq -2x^4 $}
}
\LARGE{\leftline{B)}}
\Large{\leftline{$ y' - \frac{1}{xln(x)}y = xln(x) (1)$}}
\Large{\leftline{$ x > 0 $}}
\Large{\leftline{$ y(\sqrt{e}) = \frac{e}{4} $}
\leftline{$ => \frac{dy}{dx} - \frac{1}{xln(x)}y = 0 =>$}
\leftline{$ => \frac{dy}{dx} = \frac{1}{xln(x)}y =>$}
\leftline{$ => \frac{1}{y}dy = \frac{1}{xln(x)}dx =>$}
\leftline{$ ln|y| = \int \frac{1}{xln(x)}dx + c =>(2)$}
\leftline{$ u = ln(x) => du = \frac{1}{ln(x)}dx => (3)$}
\leftline{$ (2)(3) => ln|y| = \int \frac{1}{u}du + c =>$}
\leftline{$ => ln|y| = ln|u| + c =>|\frac{y}{u}| = e^c =^{(K = \pm e^c )}=>$}
\leftline{$ => \frac{y}{u} = K => y = Ku =>$}
\leftline{$ y_0 = Ku => y = k(x)u => y = k(x)lnx =>(4)$}
\leftline{$ y' = k'(x)lnx + k(x)\frac{1}{x} => (5)$}
\leftline{$ (1)(5) => \frac{1}{xln(x)}y + xln(x) = k'(x)lnx + k(x)\frac{1}{x} =>(6) $}
\leftline{$ (4)(6) => \frac{k(x)lnx}{xln(x)} + xln(x) = k'(x)lnx + k(x)\frac{1}{x} =>$}
\leftline{$ => \frac{k(x)}{x} + xln(x) = k'(x)lnx + \frac{k(x)}{x} =>$}
\leftline{$ => xln(x) = k'(x)lnx =>$}
\leftline{$ => x = k'(x) =>$}
\leftline{$ => k(x) = \frac{x^2}{2} + c_2 =^{(4)}=>$}
\leftline{$ => y = (\frac{x^2}{2} + c_2)lnx $}
}
\LARGE{\centerline{Exercise 3.}}
\LARGE{\leftline{A)}}
\Large{\leftline{$ y' + y = 1 (1)$}} 
\Large{\leftline{$ y(0) = 0 (2) $}}
\Large{\leftline{$ y' + y = 0 => \frac{dy}{dx} = -y =^{( y \ne 0 )( x \ne 0 )}=> -\frac{1}{y}dy = dx => $}
\leftline{$ => -ln|y| = x + c => y = \pm e^{-c}e^{-x}=^{(\pm e^{-c} = K)} => $}
\leftline{$ => y = x + c => y = \pm e^{-c}e^{-x} =^{(\pm e^{-c} = K)} => $}
\leftline{$ => y = Ke^{-x} => y = K\frac{1}{e^{x}} => $}
\leftline{$ y_0 = K\frac{1}{e^{x}} = Ke^{-x} => (3)$}
\leftline{$ (y_p = c_2)(y'_p = 0)(1) => 0 + c_2 = 1 => c_2 = 1 => (4)$}
\leftline{$ (3)(4) => y = Ke^{-x} + 1 => (5)$}
\leftline{$ (2)(5) => 0 = Ke^{0} + 1 => 0 = K + 1 => K = -1 => (6) $}
\leftline{$ (5)(6) => y = -e^{-x} + 1 $}
}
\LARGE{\leftline{B)}}
\Large{\leftline{$ y' + 2y = e^x (1)$}}
\Large{\leftline{$ ( p(x) = 2 ) ( g(x) = e^x ) $}
\leftline{$ m(x) = e^{ \int p(x) dx } = e^{ \int 2 dx } = e^{ 2x }$}
\leftline{$ (1) => e^{ 2x }y' + 2e^{ 2x }y = e^{ 3x } => $}
\leftline{$ => (e^{ 2x }y)' = e^{ 3x } => e^{ 2x }y = \int e^{ 3x } dx => $}
\leftline{$ => e^{ 2x }y = \frac{e^{ 3x }}{3} + c => $}
\leftline{$ => y = \frac{e^{ x }}{3} + \frac{c}{e^{ 2x }} $}
}
\LARGE{\centerline{Exercise 4.}}
\Large{\leftline{$ y' + xy = \frac{x}{y^3} (1)$}} 
\Large{\leftline{$ y(0) = 2 (2) $}}
\Large{\leftline{$ (1) => y' + xy = \frac{x}{y^3} => y'y^3 + xy^4 = x =>  $} 
\leftline{$ => 4y'y^3 + 4xy^4 = 4x => (3) $}
\leftline{$ ( u = y^4 )( \frac{du}{dx} = 4y^3\frac{dy}{dx} => u' = 4y^3y' ) (4) $}
\leftline{$ (3)(4) => u' + 4xu = 4x (5) $}
\leftline{$ p(x) = g(x) = 4x $}
\leftline{$ m(x) = e^{ \int p(x) dx } = e^{ \int 4x dx } = e^{ 2x^2 } =>(6)$}
\leftline{$ (5)(6) => u'e^{ 2x^2 } + 4xe^{ 2x^2 }u = 4xe^{ 2x^2 } => $}
\leftline{$ => (ue^{ 2x^2 })' = (e^{ 2x^2 })' => $}
\leftline{$ => ue^{ 2x^2 } = e^{ 2x^2 } + c => $}
\leftline{$ => u = 1 + \frac{c}{e^{ 2x^2 }} => $}
\leftline{$ => y^4 = 1 + \frac{c}{e^{ 2x^2 }} => $}
\leftline{$ => y = \sqrt{1 + \frac{c}{e^{ 2x^2 }}}^4 => (7)$}
\leftline{$ (2)(7) => \sqrt{1 + \frac{c}{e^{ 0 }}}^4 = 2 => $}
\leftline{$ => \sqrt{1 + c}^4 = 2 => 1 + c = 16 => c = 15 =>(8) $}
\leftline{$(7)(8) => y = \sqrt{1 + \frac{15}{e^{ 2x^2 }}}^4 $}
} 
\end{document}